Some text.

theories/Sorting.v
@@ -13,50 +13,97 @@ Unset Printint Implicit Defensive.
 Section Sorting.
 (* end hide *)
 
-Inductive trace (n : nat) : Type :=
-| Compare (i j : 'I_n) (tl tr : trace n)
+(** In this post, we will formalize one of the most well-known results
+of algorithm analysis: no comparison sort can run in less than [O(n *
+log n)] steps when sorting an array of size [n].
+
+First, we must define a convenient datatype for representing the
+execution of a sorting algorithm. For our purposes, a sorting
+algorithm can be seen as a binary tree: internal nodes denote a
+comparison between two elements, with the right and left branches
+telling how to proceed on each case. The leaves of the tree signal
+that the algorithm halted, producing a result. This results in the
+following type: *)
+
+Inductive sort_alg (n : nat) : Type :=
+| Compare (i j : 'I_n) (l r : sort_alg n)
 | Done of 'S_n.
 
-Section Correctness.
+(** Let's analyze this declaration in detail. The [n] parameter will
+be used later to track the length of the array that we are
+sorting. ['I_n] and ['S_n] are types defined in Ssreflect: the former
+is the type of natural numbers bounded by [n], whereas the latter
+represents permutations of that type. The idea is that, when running
+our algorithm, the [i] and [j] arguments of [Compare] tell which
+elements of our array to compare. The permutation in [Done] specifies
+how to rearrange the elements of the input array to produce an
+answer. We can formalize the previous description in the following
+function: *)
 
-Variables (T : eqType) (le : rel T).
-
-Fixpoint execute n (t : trace n) (xs : n.-tuple T) : n.-tuple T :=
-  match t with
+Fixpoint execute T n c (a : sort_alg n) (xs : n.-tuple T) :=
+  match a with
+  | Compare i j l r =>
+    let a' := if c (tnth xs i) (tnth xs j) then l else r in
+    execute c a' xs
   | Done p => [tuple tnth xs (p i) | i < n]
-  | Compare i j tl tr =>
-    if le (tnth xs i) (tnth xs j) then execute tr xs
-    else execute tl xs
   end.
 
-End Correctness.
+(** [execute] is a polymorphic function that works for any type [T]
+with a comparison operator [c]. Given an algorithm [a] and an input
+array [xs] of length [n], the function compares the elements of [a],
+following the appropriate branches along the way, until finding out
+how to rearrange [a]'s elements.
 
-Definition trace_ok (t : forall n, trace n) :=
+With [execute], we can now define what it means for a sorting
+algorithm to be correct: *)
+
+Definition sort_alg_ok (a : forall n, sort_alg n) :=
   forall (T : eqType) (le : rel T),
-    transitive le ->
-    forall n xs, execute le (t n) xs =
-                 sort le xs :> seq T.
+  forall n xs, execute le (a n) xs = sort le xs :> seq T.
 
-Fixpoint comparisons n (t : trace n) : nat :=
-  match t with
-  | Compare _ _ tl tr => (maxn (comparisons tl) (comparisons tr)).+1
-  | Done _ => 0
-  end.
+(** With [sort_alg_ok] in hand, we are ready to formulate our main
+result. Informally, our proof works as follows:
+
+  - In the worst case, an array of size [n] has [n!] permutations.
+
+  - A sorting algorithm can distinguish at most [2 ^ k] permutations,
+    where [k] is the maximum number of comparisons performed.
+
+  - Therefore, [n! <= 2 ^ k], implying [log_2 n! <= k].
+
+  - Using Stirling's approximation, we can weaken this lower bound and
+    derive the final result.
+
+Unfortunately, we don't have a Coq proof of Stirling's approximation
+we can use here, which forces us to adapt the last step. We show the
+following lemma by induction ([trunc_log], as its name says, is the
+truncated logarithm): *)
 
 Local Notation log2 := (trunc_log 2).
 
 Lemma log2_fact n : (n * log2 n)./2 <= log2 n`!.
 Proof.
+(** In order to get our proof to go through, we must strengthen our
+induction hypothesis a little bit: *)
+
 suff: n * (log2 n).+2 <= (log2 n`! + 2 ^ (log2 n)).*2.+1.
+  (* ... *)
+  (* begin hide *)
   move: (leq0n n); rewrite leq_eqVlt=> /orP [/eqP <- //|pos].
   move/half_leq; rewrite -(addn1 _.*2) halfD odd_double add0n addn0 doubleK.
   rewrite -addn2 mulnDr muln2 halfD odd_double andbF doubleK add0n.
   rewrite (addnC (log2 _)) -leq_subLR -addnBA ?trunc_logP //.
   exact/leq_trans/leq_addr.
+  (* end hide *)
 have [|] := boolP (3 <= n); last by case: n => [|[|[|[|]]]] //=.
 elim: n=> [|n IH] //=.
 rewrite leq_eqVlt=> /orP [/eqP <- //|lb]; move/(_ lb) in IH.
+
+(** On the inductive step, we also have two cases to consider: whether
+or not [log2 n] is less than [log2(n.+1)]. *)
 have: log2 n.+1 = log2 n \/ log2 n.+1 = (log2 n).+1 /\ 2 ^ (log2 n.+1) = n.+1.
+(* ... *)
+(* begin hide *)
   move: (@trunc_log_bounds 2 _ erefl (@leq_trans 3 1 n erefl lb))
         (@trunc_log_bounds 2 _ erefl (@leq_trans 4 1 n.+1 erefl lb))
         => /andP [e1 e2] /andP [e3 e4].
@@ -81,37 +128,46 @@ rewrite -addnA (addnA _.+1) (addnC _.+1) 2!addnA -addnA doubleD leq_add //.
   rewrite (leq_trans (leq_add (leqnn _) lb1)) // -addnA addnn -doubleD.
   by rewrite addnC leq_double.
 by rewrite -addnn leq_add2l.
+(* end hide *)
 Qed.
 
-Import GroupScope.
+Fixpoint comparisons n (a : sort_alg n) : nat :=
+  match a with
+  | Compare _ _ l r => (maxn (comparisons l) (comparisons r)).+1
+  | Done _ => 0
+  end.
 
-Lemma trace_ok_leq n t : trace_ok t -> (n * log2 n)./2 <= comparisons (t n).
+(* begin hide *)
+Import GroupScope.
+(* end hide *)
+Lemma sort_alg_ok_leq n a :
+  sort_alg_ok a -> (n * log2 n)./2 <= comparisons (a n).
 Proof.
-move/(_ _ _ leq_trans n); move: {t} (t n) => t t_ok.
-suff lb: n`! <= 2 ^ comparisons t.
+move/(_ _ _ n); move: {a} (a n) => a a_ok.
+suff lb: n`! <= 2 ^ comparisons a.
   rewrite (leq_trans (log2_fact n)) // -(@leq_exp2l 2) //.
   by rewrite (leq_trans (trunc_logP (leqnn 2) (fact_gt0 n))).
-pose fix ps t : {set 'S_n} :=
-  match t with
-  | Compare _ _ tl tr => ps tl :|: ps tr
+pose fix ps a : {set 'S_n} :=
+  match a with
+  | Compare _ _ l r => ps l :|: ps r
   | Done p => [set p]
   end.
-have ub: #|ps t| <= 2 ^ comparisons t.
-  elim: {t_ok} t=> [i j tl IHl tr IHr|p] /=; last by rewrite cards1.
-  rewrite (leq_trans (leq_of_leqif (leq_card_setU (ps tl) (ps tr)))) //.
+have ub: #|ps a| <= 2 ^ comparisons a.
+  elim: {a_ok} a=> [i j l IHl r IHr|p] /=; last by rewrite cards1.
+  rewrite (leq_trans (leq_of_leqif (leq_card_setU (ps l) (ps r)))) //.
   by rewrite expnS mul2n -addnn leq_add // ?(leq_trans IHl, leq_trans IHr) //
      leq_exp2l // ?(leq_maxl, leq_maxr).
 rewrite (leq_trans _ ub) // {ub} -{1}(card_ord n) -cardsT -card_perm.
 rewrite -(cardsE (perm_on [set: 'I_n])) subset_leq_card //.
-apply/subsetP=> /= p _; move: {t_ok} (t_ok [tuple val (p^-1 i) | i < n]).
+apply/subsetP=> /= p _; move: {a_ok} (a_ok _ leq [tuple val (p^-1 i) | i < n]).
 rewrite (_ : sort _ _ = [tuple val i | i < n]); last first.
   apply: (eq_sorted leq_trans anti_leq (sort_sorted leq_total _)).
     by rewrite /= val_enum_ord iota_sorted.
   rewrite (perm_eq_trans (introT perm_eqlP (perm_sort _ _))) //.
   apply/tuple_perm_eqP; exists p^-1; congr val; apply/eq_from_tnth=> i.
   by rewrite 3!tnth_map 2!tnth_ord_tuple.
-elim: t=> [/= i j tl IHl tr IHr|p'].
-  by case: ifP=> [_ /IHr|_ /IHl]; rewrite in_setU => -> //; rewrite orbT.
+elim: a=> [/= i j l IHl r IHr|p'].
+  by case: ifP=> [_ /IHl|_ /IHr]; rewrite in_setU => -> //; rewrite orbT.
 move/val_inj=> /= {ps}.
 rewrite in_set1=> e; apply/eqP/permP=> i; apply/esym/(canRL (permKV p)).
 apply/val_inj.
